simplify map values

src/c0/dyn.lean
@@ -44,15 +44,12 @@ def at_nth' (R : value → value → Prop) : ℕ → value → value → Prop
 inductive at_nth (R : value → value → Prop) (i : ℕ) : value → value → Prop
 | mk {} {v v' n} : i < n → at_nth' R i v v' → at_nth (arr n v) (arr n v')
 
-inductive at_name (R : value → value → Prop) (f : ident) : value → value → Prop
-| mk {} {v v'} : R v v' → at_name (named f v) (named f v')
+def of_map (vs : alist ident (λ _, value)) : value :=
+alist.rec' nil (λ vs x v _, cons (named x v)) vs
 
 inductive at_field (R : value → value → Prop) (f : ident) : value → value → Prop
-| mk {} {v v' n} : at_nth' (at_name R f) n v v' → at_field v v'
-
-inductive is_field (f : ident) : value → value → Prop
-| one {} {v vs} : is_field (cons (named f v) vs) v
-| cons {v' v vs} : is_field vs v → is_field (cons v' vs) v
+| mk {} {v v' vs x y} : R x y → x ∈ alist.lookup f vs →
+  v = of_map vs → v' = of_map (vs.replace f y) → at_field v v'
 
 inductive is_nth : ℕ → value → value → Prop
 | zero {} {v vs} : is_nth 0 (cons v vs) v
@@ -123,8 +120,8 @@ inductive get (h : heap) (η : vars) : addr → value → Prop
 | tail {a v vs} : get a (value.cons v vs) → get (tail a) vs
 | nth {a i n v v'} : get a (value.arr n v) →
   value.is_nth i v v' → get (nth a i) v'
-| field {a f v' v} :
-  get a v' → value.is_field f v' v → get (field a f) v
+| field {a f vs v} :
+  get a (value.of_map vs) → v ∈ vs.lookup f → get (field a f) v
 
 inductive get_len (h : heap) (η : vars) : addr → ℕ → Prop
 | mk {a n v} : get h η a (value.arr n v) → get_len a n
